updates

Veritas.BinTreePtr.fst
@@ -281,67 +281,127 @@ let rec lemma_extend_not_reachable_aux
       lemma_extend_not_reachable_aux pf d a n'    
   )
   else ()
-        
-let rec lemma_extendcut_reachable_aux (pf:ptrfn)
-                              (d1:bin_tree_node{points_to_none pf d1})
-                              (a1:bin_tree_node{is_proper_desc d1 a1 /\ 
-                                               points_to_some pf a1 (desc_dir d1 a1) /\
-                                               is_proper_desc (pointed_node pf a1 (desc_dir d1 a1)) d1})
-                              (d: bin_tree_node)
-                              (a: bin_tree_node):
-  Lemma (requires (reachable pf d a))
-        (ensures (reachable (extendcut_ptrfn pf d1 a1) d a))
-        (decreases (depth d - depth a)) = 
-  lemma_reachable_implies_desc pf d a;  
-  lemma_desc_depth_monotonic d a;
-  let pfe = extendcut_ptrfn pf d1 a1 in
-  let prfda = lemma_pdesc_correct2 pf d a in
-  match prfda with
-  | PSelf _ _ -> 
-    assert(d == a);
-    lemma_reachable_reflexive pfe a
-  | PTran _ _ d' prfdd' _ c ->
-    assert(points_to pf d' a);
-    lemma_proper_desc_depth_monotonic d' a;
-    lemma_pdesc_correct pf d d' prfdd';
-    assert(reachable pf d d');
-    
-    lemma_reachable_implies_desc pf d d';
-    lemma_desc_depth_monotonic d d';
-    lemma_extendcut_reachable_aux pf d1 a1 d d';
-    assert(reachable pfe d d');             
 
-    let c1 = desc_dir d1 a1 in
-    let d2 = pointed_node pf a1 c1 in
-    let c' = desc_dir d' a in
-    if a1 = a && c1 = c' then (
-      assert(points_to pfe d1 a);
-      lemma_points_to_reachable pfe d1 a;
-      assert(reachable pfe d1 a);
-      assert(points_to pfe d' d1);
-      lemma_points_to_reachable pfe d' d1;
-      lemma_reachable_transitive pfe d d' d1;
-      assert(reachable pfe d d1);
-      lemma_reachable_transitive pfe d d1 a
+let lemma_extend_not_reachable
+  (pf:ptrfn) 
+  (d:bin_tree_node{points_to_none pf d}) 
+  (a:bin_tree_node{is_proper_desc d a /\ 
+                   not (points_to_some pf a (desc_dir d a)) /\
+                   root_reachable pf a})
+  (n: bin_tree_node):
+  Lemma (requires (not (root_reachable pf n) /\ n <> d))
+        (ensures (not (root_reachable (extend_ptrfn pf d a) n))) = 
+  lemma_extend_not_reachable_aux pf d a n
+
+let rec lemma_extendcut_reachable_aux
+  (pf:ptrfn)
+  (d:bin_tree_node{points_to_none pf d})
+  (a:bin_tree_node{is_proper_desc d a /\ 
+                    points_to_some pf a (desc_dir d a) /\
+                    is_proper_desc (pointed_node pf a (desc_dir d a)) d /\ 
+                    root_reachable pf a})
+  (n: bin_tree_node):
+  Lemma (requires (root_reachable pf n))
+        (ensures (root_reachable (extendcut_ptrfn pf d a) n)) 
+        (decreases (depth n)) = 
+  let pfe = extendcut_ptrfn pf d a in
+  if n = Root then
+    lemma_reachable_reflexive pfe n
+  else (
+    let n' = prev_in_path pf n Root in
+    lemma_proper_desc_depth_monotonic n n';
+    lemma_extendcut_reachable_aux pf d a n';
+    assert(root_reachable pfe n');
+
+    assert(points_to pf n n');
+    if n' = a && desc_dir d a = desc_dir n n' then (
+      assert(points_to pfe d n');
+      lemma_points_to_reachable pfe d n';
+      assert(points_to pfe n d);
+      lemma_points_to_reachable pfe n d;
+      lemma_reachable_transitive pfe n d n';
+      lemma_reachable_transitive pfe n n' Root
     )
     else (
-      assert(a <> d1);
-      assert(points_to pfe d' a);
-      lemma_points_to_reachable pfe d' a;
-      assert(reachable pfe d' a);
-      lemma_reachable_transitive pfe d d' a      
+      assert(points_to pfe n n');
+      lemma_points_to_reachable pfe n n';
+      lemma_reachable_transitive pfe n n' Root
     )
+  )
+  
+let lemma_extendcut_reachable 
+  (pf:ptrfn)
+  (d:bin_tree_node{points_to_none pf d})
+  (a:bin_tree_node{is_proper_desc d a /\ 
+                    points_to_some pf a (desc_dir d a) /\
+                    is_proper_desc (pointed_node pf a (desc_dir d a)) d /\ 
+                    root_reachable pf a})
+  (n: bin_tree_node):
+  Lemma (requires (root_reachable pf n))
+        (ensures (root_reachable (extendcut_ptrfn pf d a) n)) = 
+  lemma_extendcut_reachable_aux pf d a n
 
-let lemma_extendcut_reachable (pf:ptrfn)
-                              (d1:bin_tree_node{points_to_none pf d1})
-                              (a1:bin_tree_node{is_proper_desc d1 a1 /\ 
-                                               points_to_some pf a1 (desc_dir d1 a1) /\
-                                               is_proper_desc (pointed_node pf a1 (desc_dir d1 a1)) d1})
-                              (d: bin_tree_node)
-                              (a: bin_tree_node):
-  Lemma (requires (reachable pf d a))
-        (ensures (reachable (extendcut_ptrfn pf d1 a1) d a)) = 
-  lemma_extendcut_reachable_aux pf d1 a1 d a
+let lemma_extendcut_reachable_new
+  (pf:ptrfn)
+  (d:bin_tree_node{points_to_none pf d})
+  (a:bin_tree_node{is_proper_desc d a /\ 
+                    points_to_some pf a (desc_dir d a) /\
+                    is_proper_desc (pointed_node pf a (desc_dir d a)) d /\ 
+                    root_reachable pf a}):
+  Lemma (root_reachable (extendcut_ptrfn pf d a) d) = 
+  let pfe = extendcut_ptrfn pf d a in
+  lemma_extendcut_reachable pf d a a;
+  assert(root_reachable pfe a);
+  assert(points_to pfe d a);
+  lemma_points_to_reachable pfe d a;
+  lemma_reachable_transitive pfe d a Root
+
+let rec lemma_extendcut_not_reachable_aux
+  (pf:ptrfn)
+  (d:bin_tree_node{points_to_none pf d})
+  (a:bin_tree_node{is_proper_desc d a /\ 
+                    points_to_some pf a (desc_dir d a) /\
+                    is_proper_desc (pointed_node pf a (desc_dir d a)) d /\ 
+                    root_reachable pf a})
+  (n: bin_tree_node):
+  Lemma (requires (not (root_reachable pf n) /\ n <> d))
+        (ensures (not (root_reachable (extendcut_ptrfn pf d a) n)))
+        (decreases (depth n)) = 
+  let pfe = extendcut_ptrfn pf d a in
+  if root_reachable pfe n then (
+    let n' = prev_in_path pfe n Root in
+    assert(points_to pfe n n');
+    if n' = a && desc_dir n n' = desc_dir d a then ()
+    else if n' = d then (
+      let d' = pointed_node pf a (desc_dir d a) in
+      assert(n = d');
+    
+      lemma_points_to_reachable pf d' a;
+      lemma_reachable_transitive pf d' a Root
+    )
+    else (
+      assert(points_to pf n n');
+      lemma_points_to_reachable pf n n';
+      lemma_proper_desc_depth_monotonic n n';
+      if root_reachable pf n' then 
+         lemma_reachable_transitive pf n n' Root
+      else
+        lemma_extendcut_not_reachable_aux pf d a n'
+    )
+  )
+  else ()
+
+let lemma_extendcut_not_reachable 
+  (pf:ptrfn)
+  (d:bin_tree_node{points_to_none pf d})
+  (a:bin_tree_node{is_proper_desc d a /\ 
+                    points_to_some pf a (desc_dir d a) /\
+                    is_proper_desc (pointed_node pf a (desc_dir d a)) d /\ 
+                    root_reachable pf a})
+  (n: bin_tree_node):
+  Lemma (requires (not (root_reachable pf n) /\ n <> d))
+        (ensures (not (root_reachable (extendcut_ptrfn pf d a) n))) = 
+  lemma_extendcut_not_reachable_aux pf d a n
 
 let rec lemma_reachable_feq_aux (pf1: ptrfn) (pf2: ptrfn) (d: bin_tree_node) (a: bin_tree_node):
   Lemma (requires (feq_ptrfn pf1 pf2 /\ reachable pf1 d a))
